\documentclass[a4paper,11pt]{article}
\usepackage[english]{babel}
\usepackage[utf8]{inputenc}
\usepackage{amsmath,amsfonts,amssymb,graphicx,float,fancyhdr,a4wide,listings,siunitx,tikz,pgfplots,parskip}
%\usepackage[dvipsnames]{xcolor}
\newlength\figureheight
\newlength\figurewidth
\setlength\figureheight{4cm}
\lstdefinestyle{mystyle}{
	showstringspaces=false,
	basicstyle=\scriptsize\ttfamily,
	frame=shadowbox,
	breaklines=true,
	numbers=left,
	commentstyle=\color{blue},
	keywordstyle=\color{blue}\textbf,
	stringstyle=\color{red}} % This is a style for lstlistings-package (for putting in matlab/C/fortran code)
\headheight=14.5pt
\pagestyle{fancy}
\fancyhead[L]{Material model}
\fancyhead[C]{\today}
\fancyhead[R]{Mikael Ã–hman}

\newcommand{\ootimes}{\overline{\otimes}}
\newcommand{\uotimes}{\underline{\otimes}}
\newcommand{\tf}[1]{\text{\boldmath $\sf #1$}}
\newcommand{\ts}[1]{\text{\boldmath $#1$}}
\newcommand{\pderiv}[2]{\frac{\partial #1}{\partial #2}}
\newcommand{\dderiv}[2]{\frac{\mathrm{d} #1}{\mathrm{d} #2}}
\newcommand{\uv}[1]{\text{\boldmath $#1$}}
\newcommand{\um}[1]{\text{\boldmath $#1$}}
%\newcommand{\uv}[1]{\underline{#1}}
%\newcommand{\um}[1]{\underline{\underline{#1}}}
\newcommand{\dev}{{\rm dev}}
\newcommand{\vol}{{\rm vol}}
\newcommand{\sym}{{\rm sym}}
\newcommand{\iso}{{\rm iso}}
\newcommand{\trial}{{\rm trial}}
\newcommand{\tr}{{\rm tr}}
\newcommand{\rmd}{{\rm d}}
\newcommand{\rme}{{\rm e}}
\newcommand{\rmm}{{\rm m}}
\newcommand{\rmp}{{\rm p}}
\newcommand{\rmT}{{\rm T}}
\newcommand{\rmH}{{\rm H}}
\newcommand{\rmt}{{\rm t}}
\newcommand{\rmth}{{\rm th}}
\newcommand{\rmthe}{{\rm th,e}}
\newcommand{\old}{{}^{\rm n}}
\newcommand{\defeq}{:=}
\providecommand{\abs}[1]{\lvert#1\rvert}

\begin{document}
Internal variables; $\ts F^\rmp$, $\rho'$, $k$ with the choice of free energy as
\begin{align*}
	\bar{\bar{\ts E}} &\defeq \frac12(\bar{\bar{\ts C}}-\ts I)\\
	\Psi &= \Psi_{\rm solid}^\rme[\ts C^\rme,\theta] + \Psi_{\rm pore}[\rho',\theta]\\
	\Psi_{\rm solid}^\rme &=  G \bar{\bar{\ts E}}_\dev\colon\bar{\bar{\ts E}}_\dev + \frac12 K_b \bar{\bar{E}}_\vol^2\\
	\Psi_{\rm pore} &= 3\left(\frac{3}{4\pi}\right)^{-\frac13} \frac{\gamma}{L_{\rm solid}\rho_t}(\rho')^{-\frac23}(1-\rho')^{\frac23}
\end{align*}
The chosen yield surface and overstress function are
\begin{align*}
	\Phi &=\frac{1}{P} \left(\left(\bar{M}_\rme\right)^2 + a \left(\hat{\bar M}_\rmm\right)^2 - (\bar\tau_y)^2\right)\\
	a &= c (1-\rho')\\
	\eta &= \left(\frac{\langle\Phi\rangle}{\tau_c}\right)^n
\end{align*}
and the temperature dependent parameters
\begin{align*}
	\bar\tau_y[\theta] &= \tau_y^\rmd \exp\left[\frac{\gamma_\rmT}{\theta}\left(1-\frac{\theta}{\theta_\rmT}\right)\right]\\
	t_\star[\theta] &= t_\star^\rmd \exp\left[\frac{\gamma_\rmt}{\theta}\left(1-\frac{\theta}{\theta_\rmt}\right)\right]
\end{align*}
with the definitions 
\begin{align*}
	\hat{\bar M}_\rmm &= \bar M_\rmm - \frac{\rho_0'}{\rho'}\sigma_s \\
	&= \bar M_\rmm - \underbrace{\frac23\left(\frac{3}{4\pi}\right)^{-\frac13} \frac{\gamma}{L_{\rm solid}}}_{B}\underbrace{\frac{\rho_0'}{(1-\rho')^{\frac13}\rho'^{\frac23}}}_{q}
\end{align*}

For the chosen yield surface we get
\begin{align*}
	\pderiv{\Phi}{\bar M_\rme} &= \frac{2}{P}\bar M_\rme\\
	\pderiv{\Phi}{\hat{\bar M}_\rmm} &= \frac{2 a}{P}\hat{\bar M}_\rmm 
\end{align*}

Introducing $d = $ \# of dimensions
\begin{align*}
	\hat{\bar{\ts\nu}} &= \pderiv{\Phi}{\hat{\bar{\ts M}}} = 
		\frac{3}{2\bar M_\rme}\pderiv{\Phi}{\bar M_\rme}\bar{\ts M}_\dev+\frac1d\pderiv{\Phi}{\hat{\bar M}_\rmm} \ts I\\
			&= \frac{3}{P}\bar{\ts M}_\dev+\frac1d\pderiv{\Phi}{\hat{\bar M}_\rmm} \ts I\\
	\bar{\bar{\ts S}} &= 2\pderiv{\Psi}{\bar{\bar{\ts C}}}\\
	\bar{\ts S} &= f^2 \bar{\bar{\ts S}}\\
	\ts S &= (\ts F^\rmp)^{-1}\cdot\bar{\ts S}\cdot(\ts F^\rmp)^{-\rmT}\\
	\bar{\ts S} &= 2G \bar{\ts E}_\dev + K_b(\bar E_\vol -d\ln[f])\ts I\\
	\bar{\ts C} &= (\ts F^\rmp)^{-\rmT}\cdot\ts C\cdot(\ts F^\rmp)^{-1}\\
	\bar{\ts M} &= \bar{\ts C}^{-1}\cdot\ts S \approx \ts S
\end{align*}

Applying backward Euler to the rate equation gives us
\begin{align*}
	\dot{\ts F}^\rmp\cdot(\ts F^\rmp)^{-1} &= \frac{1}{t_\star}\eta\hat{\bar{\ts\nu}}\\
	&\Longrightarrow\\
	(\ts F^\rmp)^{-1} &= (\old\ts F^\rmp)^{-1}\cdot\underbrace{(\ts I - \Delta\gamma\hat{\bar{\ts\nu}})}_{\ts A}\\
	&\Longrightarrow\\
	\bar{\ts C} &= \bar{\ts F}^{\rmT}\cdot\bar{\ts F} 
				 = (\ts F^\rmp)^{-\rmT} \cdot\ts C\cdot(\ts F^\rmp)^{-1} 
				 = \ts A^\rmT\cdot \bar{\ts C}^\trial\cdot\ts A
\end{align*}

We can now express the residual in terms of the scalar unknowns
\begin{align*}
    \ts R_C &= \bar{\ts C} - \ts A^\rmT\cdot\bar{\ts C}^\trial\cdot\ts A &= 0\\
	\ts R_A &= \ts A - (\ts I - \Delta\gamma\hat{\bar{\ts\nu}}) &= 0\\
	R_\rho &= \ln[\rho']-\ln[\old\rho']+\Delta\gamma\pderiv{\Phi}{\hat{\bar M}_\rmm} &= 0\\
	R_\gamma &= t^\star \Delta\gamma - \Delta t \eta &= 0
\end{align*}
where the variables would be $\underline{X} = [\rho', \Delta\gamma, \bar{\ts C}, \ts A]$

\begin{align*}
	\tf J_{C C}      &= \tf I\\
	\tf J_{C A} &= -\ts I\uotimes(\ts A^\rmT\cdot\bar{\ts C}^\trial) - (\ts A^\rmT\cdot\bar{\ts C}^\trial)\ootimes\ts I\\
	\ts J_{C \rho}   &= \ts 0\\
	\ts J_{C \gamma} &= \ts 0
\end{align*}

\begin{align*}
	\tf J_{A C}  &= \Delta\gamma\pderiv{\hat{\bar{\ts\nu}}}{\bar{\ts C}} = \frac{\Delta\gamma}{P}(3G\tf I_\dev + \frac{a K_b}{d}\ts I\otimes\ts I)\\
	\tf J_{A A} &= \tf I\\
	\ts J_{A \rho}   &= \Delta\gamma\pderiv{\hat{\bar{\ts\nu}}}{\rho'} = \Delta\gamma\frac1{P d}(a'\hat{\bar M}_\rmm - a B q')\ts I\\
	\ts J_{A \gamma} &= \hat{\bar{\ts\nu}}
\end{align*}

\begin{align*}
	\ts J_{\rho C}  &= \Delta\gamma a \frac{K_b}{P} \ts I\\
	\ts J_{\rho A}  &= \ts 0\\
	J_{\rho \rho}   &= \frac{1}{\rho'} + \frac{2\Delta\gamma}{PG}(a' \hat{\bar M}_\rmm - a B q')\\
	J_{\rho \gamma} &= \pderiv{\Phi}{\hat{\bar M}_\rmm}
\end{align*}

\begin{align*}
	\ts J_{\gamma C}  &= -\Delta t \eta' \pderiv{\Phi}{\bar{\ts C}} 
					= -\Delta t \eta' \hat{\bar{\ts\nu}}\colon\pderiv{\hat{\bar{\ts M}}}{\bar{\ts C}}
					= -\Delta t \eta' \hat{\bar{\ts\nu}}\colon\frac12 \tf L_\rme\\
	\ts J_{\gamma A} &= \ts 0\\
	J_{\gamma \rho}   &= -\Delta t \eta'\pderiv{\Phi}{\rho'}\\
	J_{\gamma \gamma} &= t_\star
\end{align*}

\section{ATS tensor}
\subsection{Elastic part for St. Venant}
Simply the elasticity tensor as in small deformations;
\begin{align*}
	\tf L^\rme &= 2 G \tf I_\dev + K_b \ts I\otimes \ts I
\end{align*}

\subsection{Plastic part}
From paper C, equation (58) and (66)
\begin{align*}
	\rmd[\ts S] =&\ \frac12((\ts F^\rmp)^{-1}\ootimes(\ts F^\rmp)^{-1})\colon \tf L^\rme \colon \rmd[\bar{\ts C}] \\
	&+ ((\old\ts F^\rmp)^{-1}\ootimes((\ts F^\rmp)^{-1}\cdot \bar{\ts S})+((\ts F^\rmp)^{-1}\cdot \bar{\ts S})\ootimes (\old \ts F^\rmp)^{-1})\colon\rmd[\ts A]
\end{align*}

\begin{align*}
	\rmd[\underline X] &= \underbrace{-\underline J^{-1}\circ\pderiv{\underline R}{\ts C}\bigg|_{\underline X}}_{\underline{\ts D}}\colon\rmd\ts C\\
	\rmd[\bar{\ts C}]  &= \tf D_C \colon\rmd[\ts C] = (\tf J^{-1})_{11}\colon((\ts F^\rmp)^{-\rmT}\ootimes(\ts F^\rmp)^{-\rmT})\colon\rmd[\ts C]\\
	\rmd[\ts A]        &= \tf D_A \colon\rmd[\ts C] = (\tf J^{-1})_{21}\colon((\ts F^\rmp)^{-\rmT}\ootimes(\ts F^\rmp)^{-\rmT})\colon\rmd[\ts C]\\
	\rmd[\rho']        &= \ts D_\rho \colon\rmd[\ts C]\\
	\rmd[\Delta\gamma] &= \ts D_\gamma \colon\rmd[\ts C]
\end{align*}

%\begin{align*}
%	\rmd[\ts A] &= -\rmd[\Delta\gamma]\hat{\bar{\ts\nu}} - \Delta\gamma\rmd[\hat{\bar{\ts\nu}}] 
%			= -\hat{\bar{\ts\nu}}\otimes\ts D_\gamma - \Delta\gamma\pderiv{\hat{\bar{\ts\nu}}}{\ts C}\colon\rmd[\ts C]\\
%	\rmd[\hat{\bar{\ts\nu}}] &= \tf I_\dev\colon\rmd[\bar{\ts C}] + \frac{2}{3G d}\ts I(a'\hat{\bar{M}}_\rmm\rmd[\rho'] + a\rmd[\hat{\bar M}_\rmm])
%\end{align*}

\end{document}
